TM/Basic/Nop.v
@@ -5,36 +5,39 @@ Section Nop.
   Variable n : nat.
   Variable sig : finType.
 
-  Definition null_action m := Vector.const (@None sig, N) m.
+  Definition null_action := Vector.const (@None sig, N) n.
 
-  Lemma tape_move_null_action m tapes :
-    tape_move_multi tapes (null_action m) = tapes.
+  Lemma tape_move_null_action tapes :
+    tape_move_multi tapes null_action = tapes.
   Proof.
-    induction tapes; cbn in *; eauto using f_equal.
+    unfold null_action, tape_move_multi.
+    apply Vector.eq_nth_iff; intros ? i <-.
+    erewrite Vector.nth_map2; eauto.
+    rewrite Vector.const_nth.
+    cbn. reflexivity.
   Qed.
 
-  Definition nop_trans := fun (p : (FinType (EqType unit)) * Vector.t (option sig) n)  => let (q,a) := p in (q, null_action n).
 
-  Definition nop : mTM sig n :=
-    Build_mTM nop_trans tt (fun _ => true).
+  Definition Nop_TM : mTM sig n :=
+    {|
+      trans := fun _ => (tt, null_action);
+      start := tt;
+      halt := fun _ => true
+    |}.
 
   Variable F : finType.
   Variable f : F.
 
-  Definition Nop := (nop; fun _ => f).
+  Definition Nop := (Nop_TM; fun _ => f).
 
-  Definition Nop_Rel : Rel (tapes sig n) (F * tapes sig n) := (@IdR _) ||_ f.
+  Definition Nop_Rel : pRel sig F n :=
+    fun tin '(yout, tout) =>
+      yout = f /\
+      tout = tin.
 
-  Lemma Nop_total : Nop ⊨c(0) Nop_Rel.
-  Proof.
-    intros ?. exists (initc nop input). cbn. firstorder.
-  Qed.
-
-  Lemma Nop_sem: Nop ⊨ Nop_Rel.
-  Proof.
-    intros ? ? ? ?. hnf. destruct i; cbn in *; now inv H.
-  Qed.
-
+  Definition Nop_Sem : Nop ⊨c(0) Nop_Rel.
+  Proof. hnf. intros t. exists (mk_mconfig tt t). cbn. auto. Qed.
+    
 End Nop.
 
 Arguments null_action {_ _}.
@@ -45,9 +48,9 @@ Arguments Nop_Rel {n sig F} (f) x y/.
 
 Ltac smpl_TM_Nop :=
   match goal with
-  | [ |- Nop _ ⊨ _] => eapply Nop_sem
-  | [ |- Nop _ ⊨c(_) _] => eapply Nop_total
-  | [ |- projT1 (Nop _) ↓ _] => eapply RealiseIn_terminatesIn, Nop_total
+  | [ |- Nop _ ⊨ _] => eapply RealiseIn_Realise; apply Nop_Sem
+  | [ |- Nop _ ⊨c(_) _] => apply Nop_Sem
+  | [ |- projT1 (Nop _) ↓ _] => eapply RealiseIn_terminatesIn, Nop_Sem
   end.
 
 Smpl Add smpl_TM_Nop : TM_Correct.
